proof/invariant-abstract/AARCH64/ArchIpc_AI.thy
@@ -219,21 +219,17 @@ lemma copy_mrs_in_user_frame[wp, Ipc_AI_2_assms]:
   "\<lbrace>in_user_frame p\<rbrace> copy_mrs t buf t' buf' n \<lbrace>\<lambda>rv. in_user_frame p\<rbrace>"
   by (simp add: in_user_frame_def) (wp hoare_vcg_ex_lift)
 
-lemma as_user_getRestart_invs[wp]: "\<lbrace>P\<rbrace> as_user t getRestartPC \<lbrace>\<lambda>_. P\<rbrace>"
+lemma as_user_getRestart_inv[wp]:
+  "as_user t getRestartPC \<lbrace>P\<rbrace>"
   by (simp add: getRestartPC_def, rule user_getreg_inv)
 
-lemma make_arch_fault_msg_invs[wp, Ipc_AI_2_assms]: "make_arch_fault_msg f t \<lbrace>invs\<rbrace>"
-  by (cases f; wpsimp)
+lemma make_arch_fault_msg_inv[wp, Ipc_AI_2_assms]:
+  "make_arch_fault_msg ft t \<lbrace>P\<rbrace>"
+  by (cases ft; wpsimp)
 
-lemma make_fault_message_inv[wp, Ipc_AI_2_assms]:
-  "make_fault_msg ft t \<lbrace>invs\<rbrace>"
-  apply (cases ft, simp_all split del: if_split)
-     apply (wp as_user_inv getRestartPC_inv mapM_wp'
-              | simp add: getRegister_def)+
-  done
-
-crunch make_fault_msg
-  for tcb_at[wp]: "tcb_at t"
+lemma make_fault_msg_inv[wp, Ipc_AI_2_assms]:
+  "make_fault_msg ft t \<lbrace>P\<rbrace>"
+  by (cases ft; wpsimp wp: as_user_inv getRestartPC_inv mapM_wp' split_del: if_split)
 
 lemma do_fault_transfer_invs[wp, Ipc_AI_2_assms]:
   "\<lbrace>invs and tcb_at receiver\<rbrace>
@@ -410,98 +406,17 @@ lemma transfer_caps_loop_valid_vspace_objs[wp, Ipc_AI_2_assms]:
         | assumption | simp split del: if_split)+
   done
 
-crunch  make_arch_fault_msg
-  for aligned[wp, Ipc_AI_2_assms]: "pspace_aligned"
-crunch  make_arch_fault_msg
-  for distinct[wp, Ipc_AI_2_assms]: "pspace_distinct"
-crunch  make_arch_fault_msg
-  for vmdb[wp, Ipc_AI_2_assms]: "valid_mdb"
-crunch  make_arch_fault_msg
-  for ifunsafe[wp, Ipc_AI_2_assms]: "if_unsafe_then_cap"
-crunch  make_arch_fault_msg
-  for iflive[wp, Ipc_AI_2_assms]: "if_live_then_nonz_cap"
-crunch  make_arch_fault_msg
-  for state_refs_of[wp, Ipc_AI_2_assms]: "\<lambda>s. P (state_refs_of s)"
-crunch  make_arch_fault_msg
-  for ct[wp, Ipc_AI_2_assms]: "cur_tcb"
-crunch  make_arch_fault_msg
-  for zombies[wp, Ipc_AI_2_assms]: "zombies_final"
-crunch  make_arch_fault_msg
-  for it[wp, Ipc_AI_2_assms]: "\<lambda>s. P (idle_thread s)"
-crunch  make_arch_fault_msg
-  for valid_globals[wp, Ipc_AI_2_assms]: "valid_global_refs"
-crunch  make_arch_fault_msg
-  for reply_masters[wp, Ipc_AI_2_assms]: "valid_reply_masters"
-crunch  make_arch_fault_msg
-  for valid_idle[wp, Ipc_AI_2_assms]: "valid_idle"
-crunch  make_arch_fault_msg
-  for arch[wp, Ipc_AI_2_assms]: "\<lambda>s. P (arch_state s)"
-crunch  make_arch_fault_msg
-  for typ_at[wp, Ipc_AI_2_assms]: "\<lambda>s. P (typ_at T p s)"
-crunch  make_arch_fault_msg
-  for irq_node[wp, Ipc_AI_2_assms]: "\<lambda>s. P (interrupt_irq_node s)"
-crunch  make_arch_fault_msg
-  for valid_reply[wp, Ipc_AI_2_assms]: "valid_reply_caps"
-crunch  make_arch_fault_msg
-  for irq_handlers[wp, Ipc_AI_2_assms]: "valid_irq_handlers"
-crunch  make_arch_fault_msg
-  for vspace_objs[wp, Ipc_AI_2_assms]: "valid_vspace_objs"
-crunch  make_arch_fault_msg
-  for global_objs[wp, Ipc_AI_2_assms]: "valid_global_objs"
-crunch  make_arch_fault_msg
-  for global_vspace_mapping[wp, Ipc_AI_2_assms]: "valid_global_vspace_mappings"
-crunch  make_arch_fault_msg
-  for arch_caps[wp, Ipc_AI_2_assms]: "valid_arch_caps"
-crunch  make_arch_fault_msg
-  for eq_ker_map[wp, Ipc_AI_2_assms]: "equal_kernel_mappings"
-crunch  make_arch_fault_msg
-  for asid_map[wp, Ipc_AI_2_assms]: "valid_asid_map"
-crunch  make_arch_fault_msg
-  for only_idle[wp, Ipc_AI_2_assms]: "only_idle"
-crunch  make_arch_fault_msg
-  for pspace_in_kernel_window[wp, Ipc_AI_2_assms]: "pspace_in_kernel_window"
-crunch  make_arch_fault_msg
-  for cap_refs_in_kernel_window[wp, Ipc_AI_2_assms]: "cap_refs_in_kernel_window"
-crunch  make_arch_fault_msg
-  for valid_objs[wp, Ipc_AI_2_assms]: "valid_objs"
-crunch  make_arch_fault_msg
-  for valid_ioc[wp, Ipc_AI_2_assms]: "valid_ioc"
-crunch  make_arch_fault_msg
-  for pred_tcb[wp, Ipc_AI_2_assms]: "pred_tcb_at proj P t"
-crunch  make_arch_fault_msg
-  for cap_to[wp, Ipc_AI_2_assms]: "ex_nonz_cap_to p"
-
-crunch  make_arch_fault_msg
-  for v_ker_map[wp, Ipc_AI_2_assms]: "valid_kernel_mappings"
- (simp: valid_kernel_mappings_def)
-
-crunch  make_arch_fault_msg
-  for obj_at[wp, Ipc_AI_2_assms]: "\<lambda>s. P (obj_at P' pd s)"
-  (wp: as_user_inv getRestartPC_inv mapM_wp'  simp: getRegister_def)
-
 lemma dmo_addressTranslateS1_valid_machine_state[wp]:
   "do_machine_op (addressTranslateS1 addr) \<lbrace> valid_machine_state \<rbrace>"
   by (wpsimp wp: dmo_valid_machine_state)
-
-crunch make_arch_fault_msg
-  for vms[wp, Ipc_AI_2_assms]: valid_machine_state
-  (wp: as_user_inv getRestartPC_inv mapM_wp'  simp: getRegister_def ignore: do_machine_op)
 
 lemma dmo_addressTranslateS1_valid_irq_states[wp]:
   "do_machine_op (addressTranslateS1 addr) \<lbrace> valid_irq_states \<rbrace>"
   by (wpsimp wp: dmo_valid_irq_states)
 
-crunch make_arch_fault_msg
-  for valid_irq_states[wp, Ipc_AI_2_assms]: "valid_irq_states"
-  (wp: as_user_inv getRestartPC_inv mapM_wp'  simp: getRegister_def ignore: do_machine_op)
-
 lemma dmo_addressTranslateS1_cap_refs_respects_device_region[wp]:
   "do_machine_op (addressTranslateS1 addr) \<lbrace> cap_refs_respects_device_region \<rbrace>"
   by (wpsimp wp: cap_refs_respects_device_region_dmo)
-
-crunch make_arch_fault_msg
-  for cap_refs_respects_device_region[wp, Ipc_AI_2_assms]: "cap_refs_respects_device_region"
-  (wp: as_user_inv getRestartPC_inv mapM_wp'  simp: getRegister_def ignore: do_machine_op)
 
 lemma setup_caller_cap_aobj_at:
   "arch_obj_pred P' \<Longrightarrow>
@@ -511,7 +426,7 @@ lemma setup_caller_cap_aobj_at:
 
 lemma setup_caller_cap_valid_arch[Ipc_AI_2_assms, wp]:
   "setup_caller_cap st rt grant \<lbrace>valid_arch_state\<rbrace>"
-  by (wpsimp wp: valid_arch_state_lift_aobj_at_no_caps[rotated -1] setup_caller_cap_aobj_at)
+  by (wpsimp wp: valid_arch_state_lift_aobj_at_no_caps[rotated -1] setup_caller_cap_tcb_at setup_caller_cap_aobj_at)
 
 lemma transfer_caps_loop_valid_arch[Ipc_AI_2_assms]:
   "\<And>slots caps ep buffer n mi.
@@ -520,7 +435,7 @@ lemma transfer_caps_loop_valid_arch[Ipc_AI_2_assms]:
          and transfer_caps_srcs caps\<rbrace>
       transfer_caps_loop ep buffer n caps slots mi
     \<lbrace>\<lambda>_. valid_arch_state\<rbrace>"
-  by (wpsimp wp: valid_arch_state_lift_aobj_at_no_caps transfer_caps_loop_aobj_at)
+  by (wpsimp wp: valid_arch_state_lift_aobj_at_no_caps transfer_caps_loop_typ_ats transfer_caps_loop_aobj_at)
 
 end
 
@@ -537,10 +452,6 @@ named_theorems Ipc_AI_3_assms
 lemma dmo_addressTranslateS1_pspace_respects_device_region[wp]:
   "do_machine_op (addressTranslateS1 addr) \<lbrace> pspace_respects_device_region \<rbrace>"
   by (wpsimp wp: pspace_respects_device_region_dmo)
-
-crunch make_fault_msg
-  for pspace_respects_device_region[wp]: "pspace_respects_device_region"
-  (wp: as_user_inv getRestartPC_inv mapM_wp'  simp: getRegister_def ignore: do_machine_op)
 
 crunch do_ipc_transfer
   for pspace_respects_device_region[wp, Ipc_AI_3_assms]: "pspace_respects_device_region"
@@ -589,7 +500,7 @@ lemma do_ipc_transfer_valid_arch[Ipc_AI_3_assms]:
   "\<lbrace>valid_arch_state and valid_objs and valid_mdb \<rbrace>
    do_ipc_transfer s ep bg grt r
    \<lbrace>\<lambda>rv. valid_arch_state\<rbrace>"
-  by (wpsimp wp: valid_arch_state_lift_aobj_at_no_caps do_ipc_transfer_aobj_at)
+  by (wpsimp wp: valid_arch_state_lift_aobj_at_no_caps dit_tcb_at do_ipc_transfer_aobj_at)
 
 end
 
